\documentclass{article}

\begin{document}

\title{Discrete Math - Extra Credit Assignment - Week 8.1} % proof by induction
\author{Dhruvan}
\date{}
\maketitle

\section*{Induction Templates}
Ind.base (n = 1): . . . \\
Ind.step (n 7 → n + 1): . . . \\


%% ------------------------ Question 1 ------------------------ %%
\section{Question}
Prove for all \({n ≥ 1: 1 + 2 + 3 + ... + n = \frac{n^2}{2} + \frac{n}{2}}\) \\ \\
% prove for n = 1
Step 1: prove for n = 1 \\
% 1 = (1^2 + 1)/2 (indent by 4 spaces)
\begin{quote}
\(1 = \frac{1^2 + 1}{2}\) \\
% 1 = 1
\(1 = 1\)
\end{quote}

% assume true for n = k
Step 2: assume true for n = k \\
% 1 + 2 + 3 ... +k = (k^2 + k)/2
\begin{quote}
\(1 + 2 + 3 + ... + k = \frac{k^2 + k}{2}\)
\end{quote}

% prove for n = k + 1
Step 3: prove for n = k + 1 \\
% right side of the page: ((k^2+k)/2) + (k + 1) (induction step)
\begin{quote}
\(1 + 2 + 3 + ... + k + (k + 1)\) \\
\(\frac{k^2 + k}{2} + (k + 1)\) (induction step) \\
% right side of the page: (k^2 + k + 2k + 2)
\(= {k^2 + k + 2k + 2}\) \\
% right side of the page: (k^2 + 3k + 2)/2
\(= \frac{k^2 + 3k + 2}{2}\) \\
% right side of the page: ((k+1)^2 + (k+1)/2)/2
\(= \frac{(k+1)^2 + (k+1)}{2}\)
\end{quote}

%% ------------------------ Question 2 ------------------------ %%
\section{Question}
Prove for all \({n ≥ 1: 1 + 3 + 5 + ... + (2n - 1) = n^2}\) \\ \\
Step 1: prove for n = 1 \\
\begin{quote}
\(1 = 1^2\) \\
\(1 = 1\)
\end{quote}

Step 2: assume true for n = k \\
\begin{quote}
\(1 + 3 + 5 + . . . + (2k - 1) = k^2\)
\end{quote}

Step 3: prove for n = k + 1 \\
\begin{quote}
\(1 + 3 + 5 + . . . + (2k - 1) + ( 2 (k + 1) - 1)\) \\
\(k^2 + (2k + 1)\) (induction step) \\
\(= k^2 + 2k + 1\) \\
\(= (k + 1)^2\)
\end{quote}

%% ------------------------ Question 3 ------------------------ %%
\section{Question}
Prove for all \({n ≥ 1: 3^n > n}\) \\ \\
Step 1: prove for n = 1 \\
\begin{quote}
\(3^1 > 1\) \\
\(3 > 1\)
\end{quote}

Step 2: assume true for n = k \\
\begin{quote}
\(3^k > k\)
\end{quote}

Step 3: prove for n = k + 1 \\
\begin{quote}
\(3^{k+1} > k + 1\) \\
\(3 \cdot 3^k > k + 1\) \\
\(3 \cdot k > k + 1\) (induction step)\\

\end{quote}

%% ------------------------ Question 4 ------------------------ %%
\section{Question}
Prove for all \({n ≥ 1: 2 + 5 + 8 + ... + (3n - 1) = \frac{n(3n + 1)}{2}}\) \\ \\
% prove for n = 1
Step 1: prove for n = 1 \\
\begin{quote}
\(2 = \frac{1(3 \cdot 1 + 1)}{2}\) \\
\(2 = 2\)
\end{quote}

% assume true for n = k
Step 2: assume true for n = k \\
\begin{quote}
\(2 + 5 + 8 + ... + (3k - 1) = \frac{k(3k + 1)}{2}\)
\end{quote}

% prove for n = k + 1
Step 3: prove for n = k + 1 \\
\begin{quote}
\(2 + 5 + 8 + ... + (3k - 1) + (3(k + 1) - 1)\) \\
\(\frac{k(3k + 1)}{2} + (3k + 3 - 1)\) (induction step) \\
\(= \frac{k(3k + 1)}{2} + 3k + 2\) \\
\(= \frac{3k^2 + k + 6k + 4}{2}\) \\
\(= \frac{3k^2 + 7k + 4}{2}\) \\
\(= \frac{(3k^2 + 3k) + (4k + 4)}{2}\) \\
\(= \frac{3k(k + 1) + 4(k + 1)}{2}\) \\
\(= \frac{(k + 1)(3k + 4)}{2}\) \\
\(= \frac{(k + 1)(3(k + 1) + 1)}{2}\)
\end{quote}


\end{document}